Theorems.v
@@ -1,0 +1,220 @@
+Require Export Fsub.Definitions.
+
+Lemma wf_typ'_from_wf_typ : forall E T,
+  wf_typ E T ->
+  wf_typ' E T.
+Proof.
+  intros.
+  induction H; eauto.
+Qed.
+
+Hint Resolve wf_typ'_from_wf_typ : core.
+
+Hint Extern 1 (wf_typ' ?E ?T) =>
+  match goal with
+  | H: wf_typ E T |- _ => apply (proj2 (proj2 (wf_typ'_from_wf_typ E T H)))
+  end : core.
+
+Lemma wf_typ_from_wf_typ' : forall E (X : atom),
+  wf_env E ->
+  wf_typ' E X ->
+  wf_typ E X.
+Proof.
+  intros.
+  inversion H0; subst; eauto.
+Qed.
+
+Hint Resolve wf_typ_from_wf_typ' : core.
+
+Hint Extern 1 (wf_typ ?E ?T) =>
+  match goal with
+  | H: wf_typ' E T |- _ => apply (proj2 (proj2 (wf_typ_from_wf_typ' E T H)))
+  end : core.
+
+(* Reflexivity *)
+
+Theorem sub_reflexivity_aux : forall E T,
+  wf_env E ->
+  wf_typ E T ->
+  sub E T T.
+Proof.
+  intros.
+  induction H0; eauto.
+  pick fresh Y excluding (L `union` dom E) and apply sub_all; auto.
+Qed.
+
+Theorem sub_reflexivity : forall E T,
+  wf_env E ->
+  wf_typ' E T ->
+  sub E T T.
+Proof.
+  intros.
+  induction H0; eauto.
+  pick fresh Y excluding (L `union` dom E) and apply sub_all; auto.
+  apply sub_reflexivity_aux; auto.
+Qed.
+
+(* Transitivity *)
+
+Lemma wf_typ_weakening : forall T E F G,
+  wf_typ (G ++ E) T ->
+  uniq (G ++ F ++ E) ->
+  wf_typ (G ++ F ++ E) T.
+Proof.
+  intros.
+  remember (G ++ E) as F'.
+  generalize dependent G.
+  induction H; intros; subst; eauto.
+  pick fresh Y excluding (L `union` dom E `union` dom F `union` dom G) and apply wf_typ_all; auto.
+  rewrite_env ((Y ~ T1 ++ G) ++ F ++ E).
+  apply H1; auto.
+  simpl_env.
+  auto.
+Qed.
+
+Lemma uniq_from_wf_env : forall E,
+  wf_env E ->
+  uniq E.
+Proof.
+  intros E H; induction H; auto.
+Qed.
+
+Lemma wf_typ_from_binds_typ : forall X U E,
+  wf_env E ->
+  binds X U E ->
+  wf_typ E U.
+Proof.
+  intros.
+  induction H.
+  - inversion H0.
+  - analyze_binds H0; rewrite_env (nil ++ X0 ~ T ++ E);
+      apply wf_typ_weakening; auto;
+      simpl_env;
+      apply uniq_from_wf_env; auto.
+Qed.
+
+Lemma type_from_wf_typ : forall E T,
+  wf_typ E T -> type T.
+Proof.
+  intros.
+  induction H; eauto.
+Qed.
+
+Lemma type_from_wf_typ' : forall E T,
+  wf_typ' E T -> type T.
+Proof.
+  intros.
+  induction H; auto.
+  apply type_all with (L := L); auto.
+  apply type_from_wf_typ with (E := E); auto.
+Qed.
+
+Lemma wf_typ'_open : forall E U T1 T2,
+  uniq E ->
+  wf_typ' E (typ_all T1 T2) ->
+  wf_typ' E U ->
+  wf_typ' E (open_tt T2 U).
+Admitted.
+
+Theorem sub_transitivity :
+  forall E, wf_env E ->
+  forall Q, wf_typ' E Q ->
+  forall S, wf_typ' E S -> sub E S Q ->
+  forall T, wf_typ' E T -> sub E Q T ->
+  sub E S T.
+Proof.
+  intros E HwfE Q HwfQ.
+  assert (W : type Q).
+  {
+    apply type_from_wf_typ' with (E := E).
+    exact HwfQ.
+  }
+  generalize dependent E.
+  remember Q as Q' in |- *.
+  generalize dependent Q'.
+  induction W; intros Q' Heq E HwfE HwfQ S HwfS SsubQ.
+  (* NTop *)
+  - subst; intros T HwfT QsubT.
+    inversion QsubT; subst; auto.
+  (* NVar *)
+  - induction SsubQ; subst; try discriminate; auto.
+    intros T HwfT QsubT.
+    apply sub_var with (U := U); auto.
+    apply IHSsubQ; auto.
+    apply wf_typ'_from_wf_typ.
+    apply wf_typ_from_binds_typ with (X := X0); auto.
+  (* NArrow *)
+  - induction SsubQ; subst; try discriminate; intros T HwfT QsubT.
+    + inversion QsubT; subst; auto.
+      apply sub_var with (U := U); auto.
+      apply IHSsubQ; auto.
+      apply wf_typ'_from_wf_typ.
+      apply wf_typ_from_binds_typ with (X := X); auto.
+    + inversion Heq; inversion QsubT; subst; auto.
+      apply sub_arrow; auto.
+      * apply IHW1 with (Q' := T1); auto.
+        -- inversion HwfQ; auto.
+        -- inversion HwfT; auto.
+        -- inversion HwfS; auto.
+      * apply IHW2 with (Q' := T2); auto.
+        -- inversion HwfQ; auto.
+        -- inversion HwfS; auto.
+        -- inversion HwfT; auto.
+  (* NAll *)
+  - induction SsubQ; subst; try discriminate; intros T HwfT QsubT.
+    + inversion QsubT; subst; auto.
+      apply sub_var with (U := U); auto.
+      apply IHSsubQ; auto.
+      apply wf_typ'_from_wf_typ.
+      apply wf_typ_from_binds_typ with (X := X); auto.
+    + inversion Heq; inversion QsubT; subst; auto.
+      pick fresh Y excluding (L `union` dom E) and apply sub_all.
+      * apply IHW with (Q' := T1); auto.
+        -- inversion HwfQ; auto.
+        -- inversion HwfT; auto.
+        -- inversion HwfS; auto.
+      * apply H0 with (X := Y) (Q' := open_tt T2 Y); auto.
+        -- apply wf_env_sub; auto.
+           inversion HwfT; auto.
+        -- apply wf_typ'_open with (T1 := T1).
+           ++ apply uniq_from_wf_env; auto.
+              apply wf_env_sub; auto.
+              inversion HwfT; auto.
+           ++ apply wf_typ'_all with (L := dom (Y ~ T4 ++ E)).
+              ** rewrite_env (nil ++ Y ~ T4 ++ E).
+                 apply wf_typ_weakening; simpl_env.
+                 --- inversion HwfQ; auto.
+                 --- apply uniq_from_wf_env.
+                     apply wf_env_sub; auto.
+                     inversion HwfT; auto.
+              ** admit.
+           ++ apply wf_typ'_var with (U := T4); auto.
+        -- apply wf_typ'_open with (T1 := S1).
+           ++ apply uniq_from_wf_env; auto.
+              apply wf_env_sub; auto.
+              inversion HwfT; auto.
+           ++ apply wf_typ'_all with (L := dom (Y ~ T4 ++ E)).
+              ** rewrite_env (nil ++ Y ~ T4 ++ E).
+                 apply wf_typ_weakening; simpl_env.
+                 --- inversion HwfS; auto.
+                 --- apply uniq_from_wf_env.
+                     apply wf_env_sub; auto.
+                     inversion HwfT; auto.
+              ** intros. admit.
+           ++ apply wf_typ'_var with (U := T4); auto.
+        -- admit.
+        -- apply wf_typ'_open with (T1 := T4).
+           ++ apply uniq_from_wf_env; auto.
+              apply wf_env_sub; auto.
+              inversion HwfT; auto.
+           ++ apply wf_typ'_all with (L := dom (Y ~ T4 ++ E)).
+              ** rewrite_env (nil ++ Y ~ T4 ++ E).
+                 apply wf_typ_weakening; simpl_env.
+                 --- inversion HwfT; auto.
+                 --- apply uniq_from_wf_env.
+                     apply wf_env_sub; auto.
+                     inversion HwfT; auto.
+              ** intros. admit.
+           ++ apply wf_typ'_var with (U := T4); auto.
+        -- admit.
+Admitted.
